AVL/mmap: refine large_free_aux 3/3
prove last lemma...
some ugly proofs (fuel=ifuel=3)...

lib_avl_common/Spec.AVL.fst
@@ -1179,7 +1179,86 @@ let lemma_delete (#a: Type)
   =
   delete_avl_aux_bst cmp t data_to_rm
 
-let lemma_delete2 (#a: Type)
+#push-options "--fuel 3 --ifuel 3 --z3rlimit 100"
+let rec lemma_delete2_remove_leftmost (#a: Type)
+  (cmp:cmp a) (t: avl a cmp) (cond : a -> bool)
+  : Lemma
+  (requires
+    forall_keys t cond /\
+    Node? t
+  )
+  (ensures (
+    let new_t, x = remove_leftmost_avl cmp t in
+    forall_keys new_t cond /\
+    cond x
+  ))
+  = match t with
+  | Node _ Leaf _ _ _ -> ()
+  | Node _ left _ _ _ ->
+      lemma_delete2_remove_leftmost cmp left cond;
+      ()
+#pop-options
+
+let lemma_delete2_rebalance (#a: Type)
+  (t: wdm a) (cond : a -> bool)
+  : Lemma
+  (requires
+    forall_keys t cond
+  )
+  (ensures (
+    let new_t = rebalance_avl t in
+    forall_keys new_t cond
+  ))
+  = ()
+
+let lemma_delete2_merge_tree (#a: Type)
+  (v: a) (l r: wdm a) (cond: a -> bool)
+  : Lemma
+  (requires
+    cond v /\
+    forall_keys l cond /\
+    forall_keys r cond
+  )
+  (ensures forall_keys (merge_tree v l r) cond)
+  = ()
+
+#push-options "--fuel 1 --ifuel 1 --z3rlimit 100"
+let lemma_delete2_aux (#a: Type)
+  (cmp:cmp a) (t: avl a cmp) (data_to_rm: a) (cond : a -> bool)
+  : Lemma
+  (requires
+    mem cmp t data_to_rm = true /\
+    forall_keys t cond /\
+    Node? t /\
+    cmp (cdata t) data_to_rm = 0
+  )
+  (ensures (
+    let new_t = delete_avl_aux0 cmp t data_to_rm in
+    forall_keys new_t cond
+  ))
+  = match t with
+  | Node data _ Leaf _ _ -> ()
+  | Node data Leaf _ _ _ -> ()
+  | Node z l r sz hz ->
+      assert (Node? r);
+      assert (mem cmp t data_to_rm = true);
+      let new_right, succ_z = remove_leftmost_avl cmp r in
+      let height_new_right = hot_wdh new_right in
+      let height_left = hot_wdh l in
+      let new_height = M.max height_left height_new_right + 1 in
+      let new_t = merge_tree succ_z l new_right in
+      assert (sot_wds new_t = sz - 1);
+      assert (hot_wdh new_t = new_height);
+      let new_t2 = rebalance_avl new_t in
+      let final_r = delete_avl_aux0 cmp t data_to_rm in
+      assert (final_r == new_t2);
+      lemma_delete2_remove_leftmost cmp r cond;
+      lemma_delete2_merge_tree succ_z l new_right cond;
+      lemma_delete2_rebalance new_t cond
+#pop-options
+
+#push-options "--fuel 3 --ifuel 3 --z3rlimit 100"
+let rec lemma_delete2 (#a: Type)
   (cmp:cmp a) (t: avl a cmp) (data_to_rm: a) (cond : a -> bool)
   : Lemma
   (requires
@@ -1190,9 +1269,20 @@ let lemma_delete2 (#a: Type)
     let new_t, b = delete_avl_aux cmp t data_to_rm in
     forall_keys new_t cond
   ))
-  = admit ()
-
-
+  = match t with
+  | Leaf -> ()
+  | Node data left right _ _ ->
+      let delta = cmp data_to_rm data in
+      if delta < 0 then begin
+        unicity_left cmp t data_to_rm;
+        lemma_delete2 cmp left data_to_rm cond
+      end else if delta > 0 then begin
+        unicity_right cmp t data_to_rm;
+        lemma_delete2 cmp right data_to_rm cond
+      end else begin
+        lemma_delete2_aux cmp t data_to_rm cond
+      end
+#pop-options
 
 (*)
 let functional_correctness (#a: Type)
